tweak + refresh dist/

dist/Config.c
@@ -19,9 +19,7 @@ bool Config_enable_quarantine_trap = true;
 
 bool Config_enable_quarantine_strict_trap = false;
 
-size_t Config_quarantine_queue_length = (size_t)1024U;
-
-size_t Config_quarantine_queue_threshold = (size_t)256U;
+size_t Config_quarantine_queue_length = (size_t)4096U;
 
 bool Config_enable_zeroing_malloc = true;
 
