dist/internal/Slots.h
@@ -8,6 +8,7 @@
 
 #include "Utils2.h"
 #include "ExternUtils.h"
+#include "Constants.h"
 #include "Bitmap5.h"
 
 uint8_t
